coq/CircuitProperties.v
@@ -2,80 +2,80 @@ Require Export Koika.Circuits.
 Require Import Koika.Common Koika.Environments Koika.Types.
 
 Section Bools.
-  Definition bool_lt b1 b2 :=
+  Definition bool_le b1 b2 :=
     b2 = false ->
     b1 = false.
 
-  Lemma bool_lt_impl b1 b2 :
-    bool_lt b1 b2 <-> (orb (negb b1) b2) = true.
+  Lemma bool_le_impl b1 b2 :
+    bool_le b1 b2 <-> (orb (negb b1) b2) = true.
   Proof.
-    destruct b1, b2; unfold bool_lt; cbn; intuition.
+    destruct b1, b2; unfold bool_le; cbn; intuition.
   Qed.
 
-  Lemma bool_lt_and :
+  Lemma bool_le_and :
     forall b1 b1' b2 b2',
-      bool_lt b1 b1' ->
-      bool_lt b2 b2' ->
-      bool_lt (andb b1 b2) (andb b1' b2').
+      bool_le b1 b1' ->
+      bool_le b2 b2' ->
+      bool_le (andb b1 b2) (andb b1' b2').
   Proof.
-    unfold bool_lt; intros.
+    unfold bool_le; intros.
     destruct b1, b2, b1', b2'; cbn;
       intuition discriminate.
   Qed.
 
-  Lemma bool_lt_and_l :
+  Lemma bool_le_and_l :
     forall b1 b1' b2,
-      bool_lt b1 b1' ->
-      bool_lt (andb b1 b2) b1'.
+      bool_le b1 b1' ->
+      bool_le (andb b1 b2) b1'.
   Proof.
-    unfold bool_lt; intros.
+    unfold bool_le; intros.
     destruct b1, b2, b1'; cbn;
       intuition discriminate.
   Qed.
 
-  Lemma bool_lt_or :
+  Lemma bool_le_or :
     forall b1 b1' b2 b2',
-      bool_lt b1 b1' ->
-      bool_lt b2 b2' ->
-      bool_lt (orb b1 b2) (orb b1' b2').
+      bool_le b1 b1' ->
+      bool_le b2 b2' ->
+      bool_le (orb b1 b2) (orb b1' b2').
   Proof.
-    unfold bool_lt; intros.
+    unfold bool_le; intros.
     destruct b1, b2, b1', b2'; cbn;
       intuition discriminate.
   Qed.
 
-  Lemma bool_lt_mux :
+  Lemma bool_le_mux :
     forall (s: bool) b1 b1' b2 b2',
-      bool_lt b1 b1' ->
-      bool_lt b2 b2' ->
-      bool_lt (if s then b1 else b2) (if s then b1' else b2').
+      bool_le b1 b1' ->
+      bool_le b2 b2' ->
+      bool_le (if s then b1 else b2) (if s then b1' else b2').
   Proof.
-    unfold bool_lt; intros.
+    unfold bool_le; intros.
     destruct s; cbn;
       intuition discriminate.
   Qed.
 
-  Lemma bool_lt_not :
+  Lemma bool_le_not :
     forall b1 b2,
-      bool_lt b1 b2 ->
-      bool_lt (negb b2) (negb b1).
+      bool_le b1 b2 ->
+      bool_le (negb b2) (negb b1).
   Proof.
-    unfold bool_lt; intros.
+    unfold bool_le; intros.
     destruct b1, b2; cbn;
       intuition discriminate.
   Qed.
 
-  Lemma bool_lt_true :
-    forall b, bool_lt b true.
+  Lemma bool_le_true :
+    forall b, bool_le b true.
   Proof.
-    unfold bool_lt; intros;
+    unfold bool_le; intros;
       destruct b; intuition discriminate.
   Qed.
 
-  Lemma bool_lt_false :
-    forall b, bool_lt false b.
+  Lemma bool_le_false :
+    forall b, bool_le false b.
   Proof.
-    unfold bool_lt; intros;
+    unfold bool_le; intros;
       destruct b; intuition discriminate.
   Qed.
 End Bools.
@@ -119,208 +119,208 @@ Section Circuits.
                               CR CSigma).
   Notation interp_circuit := (interp_circuit cr csigma).
 
-  Definition circuit_lt (c1 c2: circuit 1) :=
-    bool_lt (Bits.single (interp_circuit c1)) (Bits.single (interp_circuit c2)).
+  Definition circuit_le (c1 c2: circuit 1) :=
+    bool_le (Bits.single (interp_circuit c1)) (Bits.single (interp_circuit c2)).
 
-  Lemma interp_circuit_circuit_lt_helper_false :
+  Lemma interp_circuit_circuit_le_helper_false :
     forall c1 c2,
-      circuit_lt c1 c2 ->
+      circuit_le c1 c2 ->
       interp_circuit c2 = Ob~0 ->
       interp_circuit c1 = Ob~0.
   Proof.
-    unfold circuit_lt; intros * Hlt Heq;
+    unfold circuit_le; intros * Hlt Heq;
       destruct (interp_circuit c1) as (? & [ ]), (interp_circuit c2) as (? & []).
     inversion Heq; cbv; f_equal; apply Hlt; cbn; congruence.
   Qed.
 
-  Lemma interp_circuit_circuit_lt_helper_true :
+  Lemma interp_circuit_circuit_le_helper_true :
     forall c1 c2,
-      circuit_lt c1 c2 ->
+      circuit_le c1 c2 ->
       interp_circuit c1 = Ob~1 ->
       interp_circuit c2 = Ob~1.
   Proof.
-    unfold circuit_lt; intros * Hlt Heq;
+    unfold circuit_le; intros * Hlt Heq;
       destruct (interp_circuit c1) as (? & [ ]), (interp_circuit c2) as ([ | ] & []);
       inversion Heq; subst; cbv; f_equal; symmetry; apply Hlt; cbn; congruence.
   Qed.
 
-  Lemma circuit_lt_CAnnot :
+  Lemma circuit_le_CAnnot :
     forall s c1 c2,
-      circuit_lt c1 c2 ->
-      circuit_lt (CAnnot s c1) (CAnnot s c2).
+      circuit_le c1 c2 ->
+      circuit_le (CAnnot s c1) (CAnnot s c2).
   Proof. firstorder. Qed.
 
-  Lemma circuit_lt_CAnnot_l :
+  Lemma circuit_le_CAnnot_l :
     forall s c1 c2,
-      circuit_lt c1 c2 ->
-      circuit_lt (CAnnot s c1) c2.
+      circuit_le c1 c2 ->
+      circuit_le (CAnnot s c1) c2.
   Proof. firstorder. Qed.
 
-  Lemma circuit_lt_CAnnot_r :
+  Lemma circuit_le_CAnnot_r :
     forall s c1 c2,
-      circuit_lt c1 c2 ->
-      circuit_lt c1 (CAnnot s c2).
+      circuit_le c1 c2 ->
+      circuit_le c1 (CAnnot s c2).
   Proof. firstorder. Qed.
 
-  Lemma circuit_lt_CBundleRef :
+  Lemma circuit_le_CBundleRef :
     forall rl1 rl2 rs1 rs2 b1 b2 field1 field2 c1 c2,
-      circuit_lt c1 c2 ->
-      circuit_lt (CBundleRef rl1 rs1 b1 field1 c1) (CBundleRef rl2 rs2 b2 field2 c2).
+      circuit_le c1 c2 ->
+      circuit_le (CBundleRef rl1 rs1 b1 field1 c1) (CBundleRef rl2 rs2 b2 field2 c2).
   Proof. firstorder. Qed.
 
-  Lemma circuit_lt_CBundleRef_l :
+  Lemma circuit_le_CBundleRef_l :
     forall rl1 rs1 b1 field1 c1 c2,
-      circuit_lt c1 c2 ->
-      circuit_lt (CBundleRef rl1 rs1 b1 field1 c1) c2.
+      circuit_le c1 c2 ->
+      circuit_le (CBundleRef rl1 rs1 b1 field1 c1) c2.
   Proof. firstorder. Qed.
 
-  Lemma circuit_lt_CBundleRef_r :
+  Lemma circuit_le_CBundleRef_r :
     forall rl2 rs2 b2 field2 c1 c2,
-      circuit_lt c1 c2 ->
-      circuit_lt c1 (CBundleRef rl2 rs2 b2 field2 c2).
+      circuit_le c1 c2 ->
+      circuit_le c1 (CBundleRef rl2 rs2 b2 field2 c2).
   Proof. firstorder. Qed.
 
-  Lemma circuit_lt_CAnd :
+  Lemma circuit_le_CAnd :
     forall c1 c1' c2 c2',
-      circuit_lt c1 c1' ->
-      circuit_lt c2 c2' ->
-      circuit_lt (CAnd c1 c2) (CAnd c1' c2').
-  Proof. unfold circuit_lt; cbn; eauto using bool_lt_and. Qed.
+      circuit_le c1 c1' ->
+      circuit_le c2 c2' ->
+      circuit_le (CAnd c1 c2) (CAnd c1' c2').
+  Proof. unfold circuit_le; cbn; eauto using bool_le_and. Qed.
 
-  Lemma circuit_lt_CAnd_l :
+  Lemma circuit_le_CAnd_l :
     forall c1 c1' c2,
-      circuit_lt c1 c1' ->
-      circuit_lt (CAnd c1 c2) c1'.
-  Proof. unfold circuit_lt; cbn; eauto using bool_lt_and_l. Qed.
+      circuit_le c1 c1' ->
+      circuit_le (CAnd c1 c2) c1'.
+  Proof. unfold circuit_le; cbn; eauto using bool_le_and_l. Qed.
 
-  Lemma circuit_lt_CAnd_r :
+  Lemma circuit_le_CAnd_r :
     forall c1 c1' c2',
-      circuit_lt c1 c1' ->
+      circuit_le c1 c1' ->
       interp_circuit c2' = Ob~1 ->
-      circuit_lt c1 (CAnd c1' c2').
-  Proof. unfold circuit_lt; cbn. intros * ? ->.
+      circuit_le c1 (CAnd c1' c2').
+  Proof. unfold circuit_le; cbn. intros * ? ->.
      cbn; rewrite Bool.andb_true_r; eauto. Qed.
 
-  Lemma circuit_lt_COr :
+  Lemma circuit_le_COr :
     forall c1 c1' c2 c2',
-      circuit_lt c1 c1' ->
-      circuit_lt c2 c2' ->
-      circuit_lt (COr c1 c2) (COr c1' c2').
-  Proof. unfold circuit_lt; cbn; eauto using bool_lt_or. Qed.
+      circuit_le c1 c1' ->
+      circuit_le c2 c2' ->
+      circuit_le (COr c1 c2) (COr c1' c2').
+  Proof. unfold circuit_le; cbn; eauto using bool_le_or. Qed.
 
-  Lemma circuit_lt_CMux :
+  Lemma circuit_le_CMux :
     forall s c1 c1' c2 c2',
-      circuit_lt c1 c1' ->
-      circuit_lt c2 c2' ->
-      circuit_lt (CMux s c1 c2) (CMux s c1' c2').
+      circuit_le c1 c1' ->
+      circuit_le c2 c2' ->
+      circuit_le (CMux s c1 c2) (CMux s c1' c2').
   Proof.
-    unfold circuit_lt; cbn;
+    unfold circuit_le; cbn;
       intros; destruct (Bits.single (interp_circuit s)); eauto.
   Qed.
 
-  Lemma circuit_lt_CMux_l :
+  Lemma circuit_le_CMux_l :
     forall s c1 c2 c3,
-      (interp_circuit s = Ob~1 -> circuit_lt c1 c3) ->
-      (interp_circuit s = Ob~0 -> circuit_lt c2 c3) ->
-      circuit_lt (CMux s c1 c2) c3.
+      (interp_circuit s = Ob~1 -> circuit_le c1 c3) ->
+      (interp_circuit s = Ob~0 -> circuit_le c2 c3) ->
+      circuit_le (CMux s c1 c2) c3.
   Proof.
-    unfold circuit_lt; cbn;
+    unfold circuit_le; cbn;
       intros * Heq1 Heq2; destruct (interp_circuit s) as [ b [] ]; cbn.
     destruct b; eauto.
   Qed.
 
-  Lemma circuit_lt_CMux_r :
+  Lemma circuit_le_CMux_r :
     forall s c1 c2 c3,
-      (interp_circuit s = Ob~1 -> circuit_lt c1 c2) ->
-      (interp_circuit s = Ob~0 -> circuit_lt c1 c3) ->
-      circuit_lt c1 (CMux s c2 c3).
+      (interp_circuit s = Ob~1 -> circuit_le c1 c2) ->
+      (interp_circuit s = Ob~0 -> circuit_le c1 c3) ->
+      circuit_le c1 (CMux s c2 c3).
   Proof.
-    unfold circuit_lt; cbn;
+    unfold circuit_le; cbn;
       intros * Heq1 Heq2; destruct (interp_circuit s) as [ b [] ]; cbn.
     destruct b; eauto.
   Qed.
 
-  Lemma circuit_lt_CNot :
+  Lemma circuit_le_CNot :
     forall c1 c2,
-      circuit_lt c1 c2 ->
-      circuit_lt (CNot c2) (CNot c1).
-  Proof. unfold circuit_lt; cbn; eauto using bool_lt_not. Qed.
+      circuit_le c1 c2 ->
+      circuit_le (CNot c2) (CNot c1).
+  Proof. unfold circuit_le; cbn; eauto using bool_le_not. Qed.
 
-  Lemma circuit_lt_true :
-    forall c, circuit_lt c (CConst Ob~1).
-  Proof. unfold circuit_lt; cbn; eauto using bool_lt_true. Qed.
+  Lemma circuit_le_true :
+    forall c, circuit_le c (CConst Ob~1).
+  Proof. unfold circuit_le; cbn; eauto using bool_le_true. Qed.
 
-  Lemma circuit_lt_false :
-    forall c, circuit_lt (CConst Ob~0) c.
-  Proof. unfold circuit_lt; cbn; eauto using bool_lt_false. Qed.
+  Lemma circuit_le_false :
+    forall c, circuit_le (CConst Ob~0) c.
+  Proof. unfold circuit_le; cbn; eauto using bool_le_false. Qed.
 
-  Lemma circuit_lt_fold_right {X} :
+  Lemma circuit_le_fold_right {X} :
     forall (xs: list X) f0 f1 c0 c1,
-      circuit_lt c1 c0 ->
-      (forall x acc1 acc0, circuit_lt acc1 acc0 -> circuit_lt (f1 x acc1) (f0 x acc0)) ->
-      circuit_lt (List.fold_right f1 c1 xs) (List.fold_right f0 c0 xs).
+      circuit_le c1 c0 ->
+      (forall x acc1 acc0, circuit_le acc1 acc0 -> circuit_le (f1 x acc1) (f0 x acc0)) ->
+      circuit_le (List.fold_right f1 c1 xs) (List.fold_right f0 c0 xs).
   Proof.
     induction xs; cbn; intros * Hlt Hxlt; eauto.
   Qed.
 
-  Lemma circuit_lt_refl :
-    forall c, circuit_lt c c.
+  Lemma circuit_le_refl :
+    forall c, circuit_le c c.
   Proof. firstorder. Qed.
 
-  Lemma circuit_lt_trans :
+  Lemma circuit_le_trans :
     forall c1 c2 c3,
-      circuit_lt c1 c2 ->
-      circuit_lt c2 c3 ->
-      circuit_lt c1 c3.
+      circuit_le c1 c2 ->
+      circuit_le c2 c3 ->
+      circuit_le c1 c3.
   Proof. firstorder. Qed.
 
-  Lemma circuit_lt_opt_l :
+  Lemma circuit_le_opt_l :
     forall c1 c2,
-      circuit_lt c1 c2 ->
-      circuit_lt (lco.(lco_fn) c1) c2.
+      circuit_le c1 c2 ->
+      circuit_le (lco.(lco_fn) c1) c2.
   Proof.
-    unfold circuit_lt; intros; rewrite lco.(lco_proof); assumption.
+    unfold circuit_le; intros; rewrite lco.(lco_proof); assumption.
   Qed.
 
-  Lemma circuit_lt_opt_r :
+  Lemma circuit_le_opt_r :
     forall c1 c2,
-      circuit_lt c1 c2 ->
-      circuit_lt c1 (lco.(lco_fn) c2).
+      circuit_le c1 c2 ->
+      circuit_le c1 (lco.(lco_fn) c2).
   Proof.
-    unfold circuit_lt; intros; rewrite lco.(lco_proof); assumption.
+    unfold circuit_le; intros; rewrite lco.(lco_proof); assumption.
   Qed.
 
-  Lemma circuit_lt_willFire_of_canFire_canFire :
+  Lemma circuit_le_willFire_of_canFire_canFire :
     forall rl_name c1 (cLog: scheduler_circuit (rule_name_t := rule_name_t) R Sigma REnv) rws,
-      circuit_lt (willFire_of_canFire lco rl_name {| canFire := c1; regs := rws |} cLog) c1.
+      circuit_le (willFire_of_canFire lco rl_name {| canFire := c1; regs := rws |} cLog) c1.
   Proof.
     unfold willFire_of_canFire; intros.
-    eapply circuit_lt_trans.
-    - eapply circuit_lt_fold_right.
-      + apply circuit_lt_refl.
+    eapply circuit_le_trans.
+    - eapply circuit_le_fold_right.
+      + apply circuit_le_refl.
       + intros; rewrite !getenv_zip.
-        eapply circuit_lt_opt_l, circuit_lt_CAnd.
+        eapply circuit_le_opt_l, circuit_le_CAnd.
         * eassumption.
-        * apply circuit_lt_true.
+        * apply circuit_le_true.
     - cbn.
       induction finite_elements; cbn.
-      + apply circuit_lt_refl.
-      + apply circuit_lt_CAnd_l; eassumption.
+      + apply circuit_le_refl.
+      + apply circuit_le_CAnd_l; eassumption.
   Qed.
 End Circuits.
 
 Arguments csigma_spec {ext_fn_t Sigma} sigma csigma : assert.
 
-Ltac circuit_lt_f_equal :=
-  repeat (apply circuit_lt_CAnnot_l ||
-          apply circuit_lt_CAnnot_r ||
-          apply circuit_lt_opt_l ||
-          apply circuit_lt_opt_r ||
-          apply circuit_lt_CBundleRef_l ||
-          apply circuit_lt_CBundleRef_r ||
-          apply circuit_lt_CAnd ||
-          apply circuit_lt_COr ||
-          apply circuit_lt_CNot ||
-          apply circuit_lt_true ||
-          apply circuit_lt_false ||
-          apply circuit_lt_refl).
+Ltac circuit_le_f_equal :=
+  repeat (apply circuit_le_CAnnot_l ||
+          apply circuit_le_CAnnot_r ||
+          apply circuit_le_opt_l ||
+          apply circuit_le_opt_r ||
+          apply circuit_le_CBundleRef_l ||
+          apply circuit_le_CBundleRef_r ||
+          apply circuit_le_CAnd ||
+          apply circuit_le_COr ||
+          apply circuit_le_CNot ||
+          apply circuit_le_true ||
+          apply circuit_le_false ||
+          apply circuit_le_refl).
